proof/TPOSR/TPOSR_trans.v
@@ -14,7 +14,7 @@ Require Import Lambda.TPOSR.LeftReflexivity.
 Require Import Lambda.TPOSR.Substitution.
 Require Import Lambda.TPOSR.CtxConversion.
 Require Import Lambda.TPOSR.RightReflexivity.
-Require Import Lambda.TPOSR.Coercion.
+Require Import Lambda.TPOSR.CtxCoercion.
 Require Import Lambda.TPOSR.Equiv.
 Require Import Lambda.TPOSR.Generation.
 Require Import Lambda.TPOSR.Validity.
